make Subarray a Slice

src/Init/Data/Array/Subarray.lean
@@ -7,6 +7,7 @@ module
 
 prelude
 import Init.Data.Array.Basic
+import Init.Data.Slice.Basic
 
 set_option linter.indexVariables true -- Enforce naming conventions for index variables.
 set_option linter.missingDocs true
@@ -21,7 +22,7 @@ Subarrays can be used to avoid copying or allocating space, while being more con
 tracking the bounds by hand. The region of interest consists of every index that is both greater
 than or equal to `start` and strictly less than `stop`.
 -/
-structure Subarray (α : Type u) where
+structure SubarrayInternal (α : Type u) where
   /-- The underlying array. -/
   array : Array α
   /-- The starting index of the region of interest (inclusive). -/
@@ -42,6 +43,29 @@ structure Subarray (α : Type u) where
   -/
   stop_le_array_size : stop ≤ array.size
 
+@[inherit_doc SubarrayInternal]
+abbrev Subarray (α : Type u) := Std.Slice (SubarrayInternal α)
+
+@[always_inline, inline, expose, inherit_doc SubarrayInternal.array]
+def Subarray.array (xs : Subarray α) : Array α :=
+  xs.internalRepresentation.array
+
+@[always_inline, inline, expose, inherit_doc SubarrayInternal.start]
+def Subarray.start (xs : Subarray α) : Nat :=
+  xs.internalRepresentation.start
+
+@[always_inline, inline, expose, inherit_doc SubarrayInternal.stop]
+def Subarray.stop (xs : Subarray α) : Nat :=
+  xs.internalRepresentation.stop
+
+@[always_inline, inline, expose, inherit_doc SubarrayInternal.start_le_stop]
+def Subarray.start_le_stop (xs : Subarray α) : xs.start ≤ xs.stop :=
+  xs.internalRepresentation.start_le_stop
+
+@[always_inline, inline, expose, inherit_doc SubarrayInternal.stop_le_array_size]
+def Subarray.stop_le_array_size (xs : Subarray α) : xs.stop ≤ xs.array.size :=
+  xs.internalRepresentation.stop_le_array_size
+
 namespace Subarray
 
 /--
@@ -51,7 +75,7 @@ def size (s : Subarray α) : Nat :=
   s.stop - s.start
 
 theorem size_le_array_size {s : Subarray α} : s.size ≤ s.array.size := by
-  let {array, start, stop, start_le_stop, stop_le_array_size} := s
+  let ⟨{array, start, stop, start_le_stop, stop_le_array_size}⟩ := s
   simp [size]
   apply Nat.le_trans (Nat.sub_le stop start)
   assumption
@@ -102,7 +126,9 @@ Examples:
 -/
 def popFront (s : Subarray α) : Subarray α :=
   if h : s.start < s.stop then
-    { s with start := s.start + 1, start_le_stop := Nat.le_of_lt_succ (Nat.add_lt_add_right h 1) }
+    ⟨{ s.internalRepresentation with
+        start := s.start + 1,
+        start_le_stop := Nat.le_of_lt_succ (Nat.add_lt_add_right h 1) }⟩
   else
     s
 
@@ -111,12 +137,13 @@ The empty subarray.
 
 This empty subarray is backed by an empty array.
 -/
-protected def empty : Subarray α where
-  array := #[]
-  start := 0
-  stop := 0
-  start_le_stop := Nat.le_refl 0
-  stop_le_array_size := Nat.le_refl 0
+protected def empty : Subarray α := ⟨{
+    array := #[]
+    start := 0
+    stop := 0
+    start_le_stop := Nat.le_refl 0
+    stop_le_array_size := Nat.le_refl 0
+  }⟩
 
 instance : EmptyCollection (Subarray α) :=
   ⟨Subarray.empty⟩
@@ -410,24 +437,24 @@ Additionally, the starting index is clamped to the ending index.
 def toSubarray (as : Array α) (start : Nat := 0) (stop : Nat := as.size) : Subarray α :=
   if h₂ : stop ≤ as.size then
     if h₁ : start ≤ stop then
-      { array := as, start := start, stop := stop,
-        start_le_stop := h₁, stop_le_array_size := h₂ }
+      ⟨{ array := as, start := start, stop := stop,
+         start_le_stop := h₁, stop_le_array_size := h₂ }⟩
     else
-      { array := as, start := stop, stop := stop,
-        start_le_stop := Nat.le_refl _, stop_le_array_size := h₂ }
+      ⟨{ array := as, start := stop, stop := stop,
+         start_le_stop := Nat.le_refl _, stop_le_array_size := h₂ }⟩
   else
     if h₁ : start ≤ as.size then
-      { array := as,
-        start := start,
-        stop := as.size,
-        start_le_stop := h₁,
-        stop_le_array_size := Nat.le_refl _ }
+      ⟨{ array := as,
+         start := start,
+         stop := as.size,
+         start_le_stop := h₁,
+         stop_le_array_size := Nat.le_refl _ }⟩
     else
-      { array := as,
-        start := as.size,
-        stop := as.size,
-        start_le_stop := Nat.le_refl _,
-        stop_le_array_size := Nat.le_refl _ }
+      ⟨{ array := as,
+         start := as.size,
+         stop := as.size,
+         start_le_stop := Nat.le_refl _,
+         stop_le_array_size := Nat.le_refl _ }⟩
 
 /--
 Allocates a new array that contains the contents of the subarray.
