src/Init/Data/Range/Polymorphic/RangeIterator.lean
@@ -7,6 +7,7 @@ module
 
 prelude
 import Init.Data.Iterators.Internal.Termination
+import Init.Data.Iterators.Consumers.Access
 import Init.Data.Iterators.Consumers.Loop
 import Init.Data.Iterators.Consumers.Collect
 import Init.Data.Range.Polymorphic.PRange
