src/Init/Data/Slice/Array.lean
@@ -10,24 +10,22 @@ import Init.Core
 import Init.Data.Range.Polymorphic.Basic
 import Init.Data.Range.Polymorphic.Nat
 import all Init.Data.Range.Polymorphic.Basic
-import Init.Data.Slice.Basic
 import Init.Data.Iterators.Combinators.Attach
 import Init.Data.Iterators.Combinators.FilterMap
 import Init.Data.Array.Subarray
+import Init.Data.Slice.Operations
 
 open Std Slice PRange
 
-abbrev Std.Slice.Subarray' (α : Type u) := Slice (Subarray α)
-
-instance {α : Type u} : Self (Slice (Subarray α)) (Subarray' α) where
+instance {α : Type u} : Self (Slice (SubarrayInternal α)) (Subarray α) where
 
 instance {shape} {α : Type u} [ClosedOpenIntersection shape Nat] :
-    Sliceable shape (Array α) Nat (Subarray' α) where
+    Sliceable shape (Array α) Nat (Subarray α) where
   mkSlice xs range :=
     let halfOpenRange := ClosedOpenIntersection.intersection range (0)...<xs.size
-    ⟨xs.toSubarray halfOpenRange.lower halfOpenRange.upper⟩
+    (xs.toSubarray halfOpenRange.lower halfOpenRange.upper)
 
-instance {s : Subarray' α} : ToIterator s Id α :=
+instance {s : Subarray α} : ToIterator s Id α :=
   .of _
     (PRange.Internal.iter (s.internalRepresentation.start...<s.internalRepresentation.stop)
       |>.attachWith (· < s.internalRepresentation.array.size) (by
