tests/lean/run/slice.lean
@@ -7,3 +7,5 @@ import Std.Data.Iterators
 #eval #[1, 2, 3][*...<2].iter.toList
 
 #eval #[1, 2, 3][1...<10].size
+
+#eval #[1, 2, 3][1...*].take 2 |>.toList
